theories/LogicalRelation/Neutral.v
@@ -23,8 +23,10 @@ Proof.
   intros; exists n.
   * eapply redtmwf_conv; tea; now eapply redtmwf_refl.
   * now eapply NeType, convneu_whne.
-  * eapply convtm_conv; [|tea].
-    now apply convtm_convneu.
+  * eapply convtm_convneu ; tea.
+    1: econstructor.
+    eapply convneu_conv; [|tea].
+    eassumption.
   * eapply RedTyRecBwd, neu. 1,2: gen_typing.
 Defined.
 
@@ -63,6 +65,24 @@ Proof.
   replace (tProd _ _) with (tProd dom cod)⟨ρ⟩ by now bsimpl.
   gen_typing.
 Qed.
+
+(* Lemma convneu_app_ren_var {Γ A f g dom cod} :
+  [Γ |- f ~ g : A] ->
+  [Γ |- A ≅ tProd dom cod] ->
+  [Γ ,, dom |- tRel 0 ≅ tRel 0 : dom⟨↑⟩] ->
+  [Γ ,, dom |- tApp f⟨↑⟩ (tRel 0) ~ tApp g⟨↑⟩ (tRel 0) : cod].
+Proof.
+  intros Hf HA Hrel.
+  erewrite <- wk1_ren_on.
+  eapply convne_meta_conv.
+  - eapply convneu_app_ren ; tea.
+    now rewrite wk1_ren_on.
+  - replace cod[_] with (cod[(0 .: ↑) >> tRel]) by now bsimpl.
+    renamify.
+    rewrite scons_eta_id'.
+    now bsimpl.
+  - now bsimpl.
+Qed. *)
 
 Record complete {l Γ A} (RA : [Γ ||-<l> A]) := {
   reflect : forall n n',
@@ -128,40 +148,133 @@ Lemma complete_Pi : forall l Γ A (RA : [Γ ||-Π< l > A]),
   complete (LRPi' RA).
 Proof.
 intros l Γ A ΠA0 ihdom ihcod; split.
-- set (ΠA := ΠA0); destruct ΠA0 as [dom cod].
-  simpl in ihdom, ihcod.
-  assert [Γ |- A ≅ tProd dom cod] by gen_typing.
-  unshelve refine ( let funred : forall n, [Γ |- n : A] -> [Γ |- n ~ n : A] -> [Γ ||-Π n : A | ΠA] := _ in _).
+set (ΠA := ΠA0); destruct ΠA0 as [dom cod].
+simpl in ihdom, ihcod.
+assert [Γ |- A ≅ tProd dom cod] by gen_typing.
+
+assert [Γ |- dom].
+{
+  erewrite <- wk_id_ren_on.
+  eapply escape, polyRed.
+  gen_typing.
+}
+assert [|- Γ ,, dom] as Hext by gen_typing.
+assert [Γ,, dom |-[ ta ] tRel 0 : dom⟨@wk1 Γ dom⟩].
+{
+  eapply ty_var ; tea.
+  rewrite wk1_ren_on.
+  econstructor.
+}
+assert [Γ,, dom |-[ ta ] tRel 0 ~ tRel 0 : dom⟨@wk1 Γ dom⟩]
+  by now apply convneu_var.
+assert [PolyRed.shpRed polyRed (wk1 dom) Hext | Γ,, dom ||- tRel 0 : dom⟨wk1 dom⟩]
+  by now eapply ihdom.
+assert [Γ ,, dom |- cod].
+{
+  replace cod with cod[tRel 0 .: @wk1 Γ dom >> tRel].
+  2: bsimpl; rewrite scons_eta'; now asimpl.
+  now eapply escape, polyRed.
+}
+assert (forall n Δ a (ρ : Δ ≤ Γ),
+    [|- Δ] -> [Γ |- n : A] -> [Δ |- a : dom⟨ρ⟩] -> [Δ |-[ ta ] tApp n⟨ρ⟩ a : cod[a .: ρ >> tRel]]) as Happ.
   {
-    intros. exists n; cbn.
-    * eapply redtmwf_refl ; gen_typing.
-    * now eapply NeFun, convneu_whne.
-    * eapply convtm_conv; [|eassumption].
-      now apply convtm_convneu.
-    * intros; apply complete_reflect_simpl; [apply ihcod| |..].
-      1: escape ; now eapply ty_app_ren.
-      eapply convneu_app_ren. 1,2: eassumption.
-      eapply LREqTermRefl_ in ha.
-      now escape.
-    * intros. apply ihcod.
-      + apply escapeTerm in ha; now eapply ty_app_ren.
-      + escape; eapply ty_conv.
-        1: now eapply ty_app_ren.
-        symmetry; unshelve eapply escapeEq, PolyRed.posExt; cycle 2; tea.
-      + apply escapeEqTerm in eq0; now eapply convneu_app_ren.
+    intros.
+    eapply typing_meta_conv.
+    1: eapply ty_app ; tea.
+    1: eapply typing_meta_conv.
+    1: eapply ty_wk.
+    - eassumption.
+    - eapply ty_conv ; tea.
+    - cbn ; reflexivity.
+    - now bsimpl. 
   }
-  intros ???? h.
-  pose proof (lrefl h); pose proof (urefl h).
-  split. 1: now apply funred.
-  unshelve econstructor.
-  1,2: now apply funred.
-  all: cbn; clear funred.
-  * gen_typing.
-  * intros. apply ihcod; cbn.
-    + apply escapeTerm in ha; now eapply ty_app_ren.
-    + apply escapeTerm in ha; now eapply ty_app_ren.
-    + eapply convneu_app_ren. 1,2: eassumption.
-    eapply escapeEqTerm; eapply LREqTermRefl_; eassumption.
+  assert (forall n, [Γ |- n : A] -> [Γ,, dom |-[ ta ] tApp n⟨@wk1 Γ dom⟩ (tRel 0) : cod]).
+  {
+    intros.
+    eapply typing_meta_conv.
+    1: apply Happ ; tea.
+    bsimpl. rewrite scons_eta'. now bsimpl.
+  }
+assert (forall n n',
+  [Γ |- n : A] -> [Γ |- n' : A] -> [Γ |- n ~ n' : A] -> [Γ |-[ ta ] n ≅ n' : tProd dom cod]).
+{
+  intros.
+  eapply convtm_eta ; tea.
+  - now eapply ty_conv.
+  - econstructor.
+    now eapply convneu_whne.
+  - now eapply ty_conv.
+  - econstructor.
+    symmetry in H19.
+    now eapply convneu_whne.
+  - eapply convneu_app_ren in H19 ; tea ; cycle -1.
+    2: eapply ihcod in H19 as [_ hred].
+    + now eapply escapeEqTerm, LREqTermRefl_.
+    + erewrite <- wk1_ren_on.
+      eapply convtm_meta_conv.
+      1: now escape.
+      1: bsimpl; rewrite scons_eta' ; now bsimpl.
+      now bsimpl.
+    + eapply typing_meta_conv ; eauto.
+      bsimpl. rewrite scons_eta'. now bsimpl.
+    + eapply typing_meta_conv ; eauto.
+      bsimpl. rewrite scons_eta'. now bsimpl.
+}
+unshelve refine ( let funred : forall n, [Γ |- n : A] -> [Γ |- n ~ n : A] -> [Γ ||-Π n : A | ΠA] := _ in _).
+{
+  intros.
+  exists n; cbn.
+  - eapply redtmwf_refl ; gen_typing.
+  - now eapply NeFun, convneu_whne.
+  - eauto.
+  - intros.
+    eapply ihcod ; last first.
+    + eapply convne_meta_conv.
+      1: eapply convneu_app.
+      * eapply convne_meta_conv.
+        1: eapply convneu_wk.
+        2: eapply convneu_conv ; tea.
+        all: cbn ; easy.
+      * now eapply escapeEqTerm, LREqTermRefl_.
+      * now bsimpl.
+      * reflexivity. 
+    + eapply Happ ; tea.
+      now escape.
+    + eapply Happ ; tea.
+      now escape.
+  - intros.
+    eapply ihcod ; last first.
+    + eapply convne_meta_conv.
+      1: eapply convneu_app.
+      * eapply convne_meta_conv.
+        1: eapply convneu_wk.
+        2: eapply convneu_conv ; tea.
+        all: cbn ; easy.
+      * now escape.
+      * now bsimpl.
+      * reflexivity. 
+    + eapply ty_conv.
+      1: eapply Happ ; tea ; now escape.
+      symmetry.
+      eapply escapeEq, PolyRed.posExt ; tea.
+    + eapply Happ ; tea.
+      now escape.
+}
+intros ???? h.
+pose proof (lrefl h); pose proof (urefl h).
+split. 1: now apply funred.
+unshelve econstructor.
+1,2: now apply funred.
+all: cbn ; clear funred.
+* eauto.
+* intros. apply ihcod; cbn.
+  + apply escapeTerm in ha; now eapply ty_app_ren.
+  + apply escapeTerm in ha; now eapply ty_app_ren.
+  + eapply convneu_app_ren. 1,2: eassumption.
+  eapply escapeEqTerm; eapply LREqTermRefl_; eassumption.
+
+Unshelve.
+all: eauto.
 Qed.
 
 Arguments ParamRedTy.outTy /.
@@ -174,61 +287,153 @@ Lemma complete_Sig : forall l Γ A (RA : [Γ ||-Σ< l > A]),
         complete (PolyRed.posRed RA ρ h ha)) ->
   complete (LRSig' RA).
 Proof.
-  intros l Γ A PA ihdom ihcod.
-  assert [Γ |- A ≅ PA.(outTy)] by (destruct PA; cbn in *; gen_typing).
-  assert [Γ |- PA.(outTy)] by (destruct PA; cbn in *; gen_typing). 
-  split.
-  - 
-    unshelve refine ( let funred : forall n, [Γ |- n : A] -> [Γ |- n ~ n : A] -> [Γ ||-Σ n : A | PA] := _ in _).
+  intros l Γ A ΣA0 ihdom ihcod.
+  set (ΣA := ΣA0); destruct ΣA0 as [dom cod] ; cbn in *.
+
+  assert [Γ |- A ≅ ΣA.(outTy)]
+    by (destruct ΣA; cbn in *; gen_typing).
+  assert [Γ |- ΣA.(outTy)]
+    by (destruct ΣA; cbn in *; gen_typing).
+  assert [Γ |- dom].
+  {
+    erewrite <- wk_id_ren_on.
+    eapply escape, polyRed.
+    gen_typing.
+  } 
+  assert [|- Γ ,, dom] as Hext by gen_typing.
+  assert [Γ,, dom |-[ ta ] tRel 0 : dom⟨@wk1 Γ dom⟩].
+  {
+    eapply ty_var ; tea.
+    rewrite wk1_ren_on.
+    econstructor.
+  }
+  assert [Γ,, dom |-[ ta ] tRel 0 ~ tRel 0 : dom⟨@wk1 Γ dom⟩]
+    by now apply convneu_var.
+  assert [PolyRed.shpRed polyRed (wk1 dom) Hext | Γ,, dom ||- tRel 0 : dom⟨wk1 dom⟩]
+    by now eapply ihdom.
+  assert [Γ ,, dom |- cod].
+  {
+    replace cod with cod[tRel 0 .: @wk1 Γ dom >> tRel].
+    2: bsimpl; rewrite scons_eta'; now asimpl.
+    now eapply escape, polyRed.
+  }
+  assert (hfst : forall n Δ (ρ : Δ ≤ Γ) (h : [ |- Δ]), [Γ |- n : A] -> [Γ |- n ~ n : A] ->
+    [PolyRedPack.shpRed ΣA ρ h | Δ ||- tFst n⟨ρ⟩ : _]).
     1:{
-      intros n **.
-      assert (hfst : forall Δ (ρ : Δ ≤ Γ) (h : [ |- Δ]), [PolyRedPack.shpRed PA ρ h | Δ ||- tFst n⟨ρ⟩ : _]).
-      1:{
-        intros; eapply complete_reflect_simpl.
-        * eapply ihdom.
-        * rewrite wk_fst; eapply ty_wk; tea.
-          eapply ty_fst; now eapply ty_conv.
-        * rewrite wk_fst; eapply convneu_wk; tea.
-          eapply convneu_fst; now eapply convneu_conv.
-      }
-      exists n hfst.
-      + eapply redtmwf_refl; now eapply ty_conv.
-      + constructor; now eapply convneu_whne.
-      + eapply convtm_convneu; now eapply convneu_conv.
-      + intros; irrelevanceRefl.
-        eapply complete_reflect_simpl; [unshelve eapply ihcod|..]; tea.
-        1: eapply hfst.
-        all: rewrite wk_fst; rewrite <- subst_ren_subst_mixed; rewrite wk_snd.
-        * eapply ty_wk; tea; eapply ty_snd; now eapply ty_conv.
-        * eapply convneu_wk; tea; eapply convneu_snd; now eapply convneu_conv.
-    }
-    intros.
-    unshelve refine (let Rn :[Γ ||-Σ n : A | PA] := _ in _).
-    1: eapply funred; tea; now eapply lrefl.
-    unshelve refine (let Rn' :[Γ ||-Σ n' : A | PA] := _ in _).
-    1: eapply funred; tea; now eapply urefl.
-    assert (Rnn' : forall (Δ : context) (ρ : Δ ≤ Γ) (h : [ |-[ ta ] Δ]),
-      [PolyRedPack.shpRed PA ρ h | Δ ||- tFst n⟨ρ⟩ ≅ tFst n'⟨ρ⟩ : (ParamRedTyPack.dom PA)⟨ρ⟩]).
-    1:{
-      intros; cbn; eapply ihdom.
+      intros; eapply complete_reflect_simpl.
+      * eapply ihdom.
       * rewrite wk_fst; eapply ty_wk; tea.
         eapply ty_fst; now eapply ty_conv.
-      * rewrite wk_fst; eapply ty_wk; tea.
-        eapply ty_fst; now eapply ty_conv. 
-      * do 2 rewrite wk_fst; eapply convneu_wk; tea.
+      * rewrite wk_fst; eapply convneu_wk; tea.
         eapply convneu_fst; now eapply convneu_conv.
     }
+  assert (hconv_fst : forall n n' Δ (ρ : Δ ≤ Γ) (h : [ |- Δ]), [Γ |- n : A] -> [Γ |- n' : A] -> [Γ |- n ~ n' : A] ->
+    [PolyRedPack.shpRed ΣA ρ h | Δ ||- tFst n⟨ρ⟩ ≅ tFst n'⟨ρ⟩ : _]).
+    1:{
+      intros.
+      eapply ihdom.
+      * rewrite wk_fst; eapply ty_wk; tea.
+        eapply ty_fst; now eapply ty_conv.
+      * rewrite wk_fst ; eapply ty_wk ; tea.
+        eapply ty_fst ; now eapply ty_conv. 
+      * repeat rewrite wk_fst; eapply convneu_wk; tea.
+        eapply convneu_fst; now eapply convneu_conv.
+    }
+  assert (hconv : forall n n',
+  [Γ |- n : A] -> [Γ |- n' : A] -> [Γ |- n ~ n' : A] -> [Γ |-[ ta ] n ≅ n' : tSig dom cod]).
+  {
+    intros.
+    eapply convtm_eta_sig ; cbn in * ; tea.
+    - now eapply ty_conv.
+    - econstructor.
+      now eapply convneu_whne.
+    - now eapply ty_conv.
+    - econstructor.
+      symmetry in H19.
+      now eapply convneu_whne.
+    - eapply convtm_meta_conv.
+      1: eapply escapeEqTerm, ihdom.
+      4: now rewrite wk_id_ren_on.
+      4: reflexivity.
+      all: rewrite wk_id_ren_on.
+      + now eapply ty_fst, ty_conv.
+      + now eapply ty_fst, ty_conv.
+      + eapply convneu_fst, convneu_conv ; tea.
+      Unshelve.
+      gen_typing.
+    - eapply convtm_meta_conv.
+      1: eapply escapeEqTerm, (ihcod _ (tFst n) wk_id).
+      5: reflexivity.
+      Unshelve.
+      + eapply typing_meta_conv.
+        1: gen_typing.
+        now bsimpl.
+      + eapply ty_conv.
+        1: gen_typing.
+        symmetry.
+        replace (cod[(tFst n')..]) with (cod[(tFst n') .: (@wk_id Γ) >> tRel]) by (now bsimpl).
+        eapply escapeEq, polyRed.(PolyRed.posExt) ; tea.
+        Unshelve.
+        * erewrite <- wk_id_ren_on ; eapply hfst ; tea.
+          now eapply urefl.
+        * now erewrite <- (wk_id_ren_on _ n), <- (wk_id_ren_on _ n').
+        * gen_typing.
+        * erewrite <- wk_id_ren_on.
+          eapply hfst ; tea.
+          now eapply lrefl. 
+      + eapply convne_meta_conv.
+        1:now eapply convneu_snd, convneu_conv.
+        1: now bsimpl.
+        easy.
+      + now bsimpl.
+      + gen_typing.
+      + erewrite <- wk_id_ren_on.
+        eapply hfst ; tea.
+        now eapply lrefl. 
+      }
+  split.
+  unshelve refine ( let funred : forall n, [Γ |- n : A] -> [Γ |- n ~ n : A] -> [Γ ||-Σ n : A | ΣA] := _ in _).
+  {
+    intros n **.
+    cbn in *.
+    unshelve eexists n _.
+    - intros. now eapply hfst. 
+    - eapply redtmwf_refl; now eapply ty_conv.
+    - constructor; now eapply convneu_whne.
+    - eauto.
+    - intros.
+      cbn.
+      eapply complete_reflect_simpl.
+      * eapply ihcod.
+      * rewrite wk_snd.
+        eapply typing_meta_conv.
+        1: eapply ty_wk ; tea.
+        1: now eapply ty_snd, ty_conv.
+        now bsimpl.
+      * eapply convne_meta_conv.
+        3: reflexivity.
+        1: rewrite wk_snd.
+        1: eapply convneu_wk ; tea.
+        1: now eapply convneu_snd, convneu_conv.
+        now bsimpl.
+  }
+    intros.
+    unshelve refine (let Rn :[Γ ||-Σ n : A | ΣA] := _ in _).
+    1: eapply funred; tea; now eapply lrefl.
+    unshelve refine (let Rn' :[Γ ||-Σ n' : A | ΣA] := _ in _).
+    1: eapply funred; tea; now eapply urefl.
     assert (forall (Δ : context) (ρ : Δ ≤ Γ) (h : [ |-[ ta ] Δ]),
-      [Δ |- (ParamRedTy.cod PA)[tFst n⟨ρ⟩ .: ρ >> tRel] ≅ (ParamRedTy.cod PA)[tFst n'⟨ρ⟩ .: ρ >> tRel]]).
+      [Δ |- cod[tFst n⟨ρ⟩ .: ρ >> tRel] ≅ cod[tFst n'⟨ρ⟩ .: ρ >> tRel]]).
     {
-      intros; eapply escapeEq; unshelve eapply (PolyRed.posExt PA); tea.
+      intros; eapply escapeEq; unshelve eapply (PolyRed.posExt ΣA); tea.
       + eapply Rn.
       + eapply Rn'.
-      + eapply Rnn'.
+      + now eapply hconv_fst.
     }
     split; tea; eexists Rn Rn'.
-    + cbn; eapply convtm_convneu; now eapply convneu_conv.
-    + apply Rnn'.
+    + cbn.
+      now eapply hconv.
+    + cbn. intros. now eapply hconv_fst.
     + intros; cbn; eapply ihcod.
       all: rewrite wk_fst; rewrite !wk_snd.
       2: eapply ty_conv; [|now symmetry]; rewrite wk_fst.
@@ -248,6 +453,7 @@ Proof.
     1,4,5: eapply redtmwf_refl; tea; now eapply ty_conv.
     2,4: do 2 constructor; tea.
     1,4: eapply convtm_convneu.
+    1,3: now constructor.
     all: eapply convneu_conv; [|eassumption].
     all: first [assumption|now eapply lrefl].
 Qed.
@@ -262,6 +468,7 @@ Proof.
     1,4,5: eapply redtmwf_refl; tea; now eapply ty_conv.
     2,4: do 2 constructor; tea.
     1,4: eapply convtm_convneu.
+    1,3: now constructor.
     all: eapply convneu_conv; [|eassumption].
     all: try first [assumption|now eapply lrefl].
 Qed.
@@ -302,8 +509,7 @@ Proof.
   assert ([Γ |-[ ta ] n ~ n' :List ListRedTy.par LA']).
   {
     eapply convneulist_convneu, convneu_conv ; tea.
-    cbn.
-    gen_typing.
+    cbn ; gen_typing.
   }
   split.
   all: now eapply complete_List_list_neutrals.
